Updated

SysF.v
@@ -1,8 +1,8 @@
 Require Import Arith.
+Require Import Arith.Max.
+Require Import Omega.
 
-Inductive kind :=
-| star : nat -> kind
-.
+Definition kind := nat.
 
 Inductive typ :=
 | tvar : nat -> typ
@@ -78,5 +78,692 @@ Fixpoint subst_typ (t : term) (X : nat) (T : typ) {struct t} : term :=
   | app_t e1 T2 => app_t (subst_typ e1 X T) (tsubst T2 X T)
   end.
 
-Definition env : Set :=
-| 
+Inductive env : Set :=
+| empty : env
+| evar  : typ -> env -> env
+| etvar : kind -> env -> env
+.
+
+Fixpoint get_kind (e : env) (i : nat) : option kind :=
+  match e with
+    | empty => None
+    | evar _ e' => get_kind e' i
+    | etvar k e' =>
+      if beq_nat i 0
+      then Some k
+      else get_kind e' (i - 1)
+  end.
+
+Fixpoint get_typ (e : env) (i : nat) : option typ :=
+  match e with
+    | empty => None
+    | etvar _ e' => get_typ e' i
+    | evar t e' =>
+      if beq_nat i 0
+      then Some t
+      else get_typ e' (i - 1)
+  end.
+
+Fixpoint bwf_typ (e : env) (t : typ) : bool :=
+  match t with
+    | tvar x =>
+      match get_kind e x with
+        | None => false
+        | Some _ => true
+      end
+    | tarr t1 t2 => (bwf_typ e t1 && bwf_typ e t2)%bool
+    | tall k t2 => bwf_typ (etvar k e) t2
+  end.
+
+Open Scope bool.
+
+Fixpoint bwf_env (e : env) : bool :=
+  match e with
+    | empty => true
+    | evar t e => bwf_typ e t && bwf_env e
+    | etvar k e => bwf_env e
+  end.
+
+Definition wf_typ (e : env) (t : typ) : Prop :=
+  bwf_typ e t = true.
+
+Definition wf_env (e : env) : Prop :=
+  bwf_env e = true.
+
+Fixpoint kinding (e : env) (t : typ) (k : kind) : Prop :=
+  match t with
+    | tvar x =>
+      match get_kind e x with
+        | None => False
+        | Some k' => wf_env e /\ k' <= k
+      end
+    | tarr t1 t2 =>
+      exists k1 k2 : kind,
+        max k1 k2 = k /\
+        kinding e t1 k1 /\
+        kinding e t2 k2
+    | tall k1 t1 =>
+      exists k' : kind,
+        kinding (etvar k1 e) t1 k' /\
+        k = 1 + max k' k1
+  end.
+
+Fixpoint typing (e : env) (t : term) (ty : typ) : Prop :=
+  match t with
+    | var x =>
+      match get_typ e x with
+        | None => False
+        | Some ty' => wf_env e /\ ty = ty'
+      end
+    | abs ty' t' =>
+      match ty with
+        | tarr ty1 ty2 =>
+          ty1 = ty' /\
+          typing (evar ty1 e) t' ty2
+        | _ => False
+      end
+    | app t1 t2 =>
+      exists ty2 : typ,
+        typing e t1 (tarr ty2 ty) /\
+        typing e t2 ty2
+    | abs_t k t' =>
+      match ty with
+        | tall k' ty' =>
+          k' = k /\
+          typing (etvar k e) t' ty'
+        | _ => False
+      end
+    | app_t t' ty' =>
+      exists l : kind,
+        exists ty1 : typ,
+          typing e t' (tall l ty1) /\
+          kinding e ty' l /\
+          ty = tsubst ty1 0 ty'
+  end.
+
+
+Fixpoint kind_of (e : env) (t : typ) : option kind :=
+  match t with
+    | tvar x => if bwf_env e then get_kind e x else None
+    | tarr t1 t2 =>
+      match kind_of e t1 with
+        | None => None
+        | Some k1 =>
+          match kind_of e t2 with
+            | None => None
+            | Some k2 => Some (max k1 k2)
+          end
+      end
+    | tall k t' =>
+      match kind_of (etvar k e) t' with
+        | None => None
+        | Some k' => Some (1 + max k k')
+      end
+  end.
+
+Fixpoint beq_typ (t1 : typ) (t2 : typ) : bool :=
+  match (t1, t2) with
+    | (tvar x, tvar y) => beq_nat x y
+    | (tarr t1 t2, tarr t1' t2') =>
+      (beq_typ t1 t1' && beq_typ t2 t2')%bool
+    | (tall k t, tall k' t') =>
+      (beq_nat k k' && beq_typ t t')%bool
+    | _ => false
+  end.
+
+Lemma beq_typ_correct : forall t1 t2 : typ, beq_typ t1 t2 = true -> t1 = t2.
+  intro.
+  induction t1.
+  + {
+      intros.
+      simpl in H.
+      destruct t2.
+      - {
+          apply eq_sym in H.
+          apply beq_nat_eq in H.
+          congruence.
+        }
+      - inversion H.
+      - inversion H.
+    }
+  + {
+      intros.
+      simpl in H.
+      destruct t2.
+      - inversion H.
+      - {
+          Require Import Bool.
+          apply andb_true_iff in H.
+          destruct H.
+          apply IHt1_1 in H.
+          apply IHt1_2 in H0.
+          congruence.
+        }
+      - inversion H.
+    }
+  + {
+      intros.
+      simpl in H.
+      destruct t2.
+      - inversion H.
+      - inversion H.
+      - {
+          Require Import Bool.
+          apply andb_true_iff in H.
+          destruct H.
+          apply IHt1 in H0.
+          apply eq_sym in H. apply beq_nat_eq in H.
+          congruence.
+        }
+    }
+Qed.
+
+Lemma beq_typ_refl : forall t : typ, beq_typ t t = true.
+  intro.
+  induction t.
+  + simpl. apply eq_sym. apply beq_nat_refl.
+  + simpl. apply andb_true_iff. split. apply IHt1. apply IHt2.
+  + simpl. apply andb_true_iff. split. apply eq_sym. apply beq_nat_refl. apply IHt.
+Qed.
+
+Fixpoint leq (m : nat) (n : nat) :=
+  match (m, n) with
+    | (O, _) => true
+    | (S m', S n') => leq m' n'
+    | (S _, O) => false
+  end.
+
+Theorem leq_prop : forall m n : nat, true = leq m n <-> m <= n.
+  intro.
+  induction m.
+  intro. simpl. split. intro. auto with arith. tauto.
+  intro. split.
+  intro. destruct n. simpl in H. inversion H. specialize (IHm n). simpl in H. apply IHm in H.
+  auto with arith.
+  intro.
+  simpl. destruct n. exfalso. apply (le_Sn_0 m). apply H.
+  assert (m <= n). omega. apply IHm. apply H0.
+Qed.
+
+Fixpoint type_of (e : env) (t : term) : option typ :=
+  match t with
+    | var x => if bwf_env e then get_typ e x else None
+    | abs ty t' =>
+      match type_of (evar ty e) t' with
+        | Some ty1 => Some (tarr ty ty1)
+        | None => None
+      end
+    | app t1 t2 =>
+      match type_of e t1 with
+        | Some (tarr ty1 ty2) =>
+          match type_of e t2 with
+            | Some ty1' =>
+              if beq_typ ty1 ty1'
+              then Some ty2
+              else None
+            | _ => None
+          end
+        | _ => None
+      end
+    | abs_t k t' =>
+      match type_of (etvar k e) t' with
+        | Some ty1 => Some (tall k ty1)
+        | None => None
+      end
+    | app_t t ty =>
+      match type_of e t with
+        | Some (tall k t') =>
+          match kind_of e ty with
+            | Some k' =>
+              if leq k' k
+              then Some (tsubst t' 0 ty)
+              else None
+            | None => None
+          end
+        | _ => None
+      end
+  end.
+
+Require Import Lt.
+(* This is not required, but makes me happy *)
+Lemma kinding_sub : forall t : typ, forall e : env, forall k1 k2 : kind,
+                      k1 <= k2 -> kinding e t k1 -> kinding e t k2.
+  intro.
+  induction t.
+  + {
+      intros.
+      simpl.
+      simpl in H0.
+      remember (get_kind e n) as k' in H0 |- *.
+      destruct k'.
+      - split. apply H0. destruct H0. omega.
+      - apply H0.
+    }
+  + {
+      intros.
+      simpl.
+      simpl in H0.
+      destruct H0. destruct H0.
+      specialize (IHt1 e x).
+      specialize (IHt2 e x0).
+      exists k2. exists k2.
+      destruct H0. destruct H0. destruct H1.
+      split. apply max_l. trivial.
+      split. apply IHt1. assert (x <= max x x0). auto with arith. omega. apply H0.
+      apply IHt2. assert (x0 <= max x x0). auto with arith. omega. apply H1.
+    }
+  + {
+      intros.
+      simpl.
+      simpl in H0. destruct H0. destruct H0.
+      exists (k2 - k1 + (max x k)). split.
+      apply (IHt (etvar k e) x). assert (x <= max x k). auto with arith. omega. apply H0.
+      assert (max x k >= k). auto with arith. assert (k2 - k1 + max x k >= k). omega.
+      assert (max (k2 - k1 + max x k) k = (k2 - k1 + max x k)). auto with arith. rewrite H4.
+      rewrite -> H1. assert (S (k2 - S (max x k) + max x k) = k2 - S (max x k) + S (max x k)).
+      omega. rewrite -> H5. assert (k2 - S (max x k) + S (max x k) = k2 - (S (max x k) - S (max x k))).
+      omega. (* THIS TAKES A WHILE *) rewrite H6. rewrite (minus_diag (S (max x k))). auto with arith.
+    }
+Qed.
+      
+Theorem kind_of_correct : forall t : typ, forall e : env,
+                            match kind_of e t with
+                              | Some k => kinding e t k
+                              | None => forall k : kind, kinding e t k -> False
+                            end.
+  intro.
+  induction t.
+  + { (* tvar *)
+      intro.
+      simpl.
+      unfold wf_env.
+      case (bwf_env e).
+      - {
+          case (get_kind e n).
+          auto.
+          auto.
+        }
+      - {
+          case (get_kind e n).
+          intros. destruct H. discriminate H. auto.
+        }
+    }
+  + { (* tarr *)
+      intro.
+      simpl.
+      specialize (IHt1 e).
+      specialize (IHt2 e).
+      remember (kind_of e t1) as k in IHt1 |- *.
+      destruct k.
+      - (* some k *) {
+         remember (kind_of e t2) as k2 in IHt2 |- *.
+          destruct k2.
+          * {
+              exists k.
+              exists k0.
+              split.
+              auto. auto.
+            }
+          * {
+              intros.
+              destruct H.
+              destruct H.
+              apply IHt2 with x0.
+              destruct H.
+              destruct H0.
+              apply H1.
+            }
+        }
+      - (* none *) {
+          intros.
+          destruct H.
+          destruct H.
+          apply IHt1 with x.
+          destruct H.
+          destruct H0.
+          apply H0.
+        }
+    }
+  + (* tall *) {
+      intro.
+      simpl.
+      specialize (IHt (etvar k e)).
+      remember (kind_of (etvar k e) t) as k' in IHt |- *.
+      destruct k'.
+      * {
+          exists k0.
+          split. apply IHt. rewrite -> max_comm. trivial.
+        }
+      * {
+          intro.
+          intro.
+          destruct H.
+          apply IHt with (k0 := x).
+          destruct H.
+          apply H.
+        }
+    }
+Qed.
+
+Lemma typing_uniq :
+  forall t : term, forall e : env, forall ty1 ty2 : typ,
+    typing e t ty1 -> typing e t ty2 -> ty1 = ty2.
+  intro.
+  induction t.
+  + {
+      intros. simpl.
+      unfold typing in H.
+      unfold typing in H0.
+      destruct (get_typ e n).
+      destruct H. destruct H0.
+      apply eq_sym in H1.
+      apply (eq_trans H2) in H1.
+      auto.
+      inversion H.
+    }
+  + {
+      intros.
+      simpl in H.
+      destruct ty1.
+      - inversion H.
+      - {
+          simpl in H0.
+          destruct ty2.
+          * inversion H0.
+          * {
+              destruct H. destruct H0.
+              apply eq_sym in H0. apply (eq_trans H) in H0.
+              apply (IHt (evar ty1_1 e) ty1_2 ty2_2) in H1.
+              congruence.
+              rewrite -> H0.
+              apply H2.
+            }
+          * inversion H0.
+        }
+      - inversion H.
+    }
+  + {
+      intros.
+      simpl in H. simpl in H0.
+      destruct H. destruct H0.
+      destruct H. destruct H0.
+      apply (IHt1 e (tarr x ty1) (tarr x ty2)) in H.
+      injection H. trivial.
+      apply (IHt2 e x x0) in H1.
+      rewrite -> H1. apply H0.
+      apply H2.
+    }
+  + {
+      intros.
+      simpl in H. simpl in H0.
+      destruct ty1.
+      - inversion H.
+      - inversion H.
+      - destruct ty2.
+        * inversion H0.
+        * inversion H0.
+        * {
+            destruct H. destruct H0.
+            apply (IHt (etvar k e) ty1 ty2) in H1.
+            congruence.
+            apply H2.
+          }
+    }
+  + {
+      intros.
+      simpl in H. simpl in H0.
+      destruct H. destruct H0.
+      destruct H. destruct H0.
+      destruct H. destruct H0. destruct H1. destruct H2.
+      apply (IHt e (tall x x1) (tall x0 x2)) in H.
+      injection H. intros.
+      rewrite H3. rewrite H4.
+      congruence.
+      apply H0.
+    }
+Qed.
+
+Lemma kind_of_minimal : forall t : typ, forall e : env, forall k : kind,
+                          match kind_of e t with
+                            | Some k' => kinding e t k -> k' <= k
+                            | None => kinding e t k -> False
+                          end.
+  intro. induction t.
+  + {
+      intros. simpl.
+      remember (bwf_env e) as wfenv.
+      remember (get_kind e n) as envkind.
+      destruct wfenv.
+      - {
+          destruct envkind.
+          * intros. destruct H. trivial.
+          * trivial.
+        }
+      - {
+          intros.
+          destruct envkind.
+          * destruct H. unfold wf_env in H. apply (eq_trans Heqwfenv) in H. inversion H.
+          * apply H.
+        }
+    }
+  + {
+      intros.
+      simpl.
+      specialize (IHt1 e). specialize (IHt2 e).
+      remember (kind_of e t1) as kind_t1 in IHt1 |- *.
+      remember (kind_of e t2) as kind_t2 in IHt2 |- *.
+      destruct kind_t1.
+      - {
+          destruct kind_t2.
+          * {
+              intro.
+              destruct H. destruct H. destruct H. destruct H0. apply IHt1 in H0. apply IHt2 in H1.
+              apply (max_case k0 k1 (fun x => x <= k)).
+              assert (x <= max x x0). auto with arith. rewrite -> H in H2. omega.
+              assert (x0 <= max x x0). auto with arith. rewrite -> H in H2. omega.
+            }
+          * intros. destruct H. destruct H. destruct H. destruct H0. apply (IHt2 x0). apply H1.
+        }
+      - intros. destruct H. destruct H. destruct H. destruct H0. apply (IHt1 x). apply H0.
+    }
+  + {
+      intros. simpl.
+      specialize (IHt (etvar k e)).
+      remember (kind_of (etvar k e) t) as kind_e in IHt |- *.
+      destruct kind_e.
+      - {
+          intros. destruct H. destruct H.
+          apply IHt in H.
+          rewrite -> H0.
+          apply le_n_S.
+          apply (max_case k k1 (fun n => n <= max x k)).
+          apply le_max_r.
+          assert (x <= max x k). apply le_max_l.
+          omega.
+        }
+      - intros. destruct H. destruct H. apply (IHt x). apply H.
+    }
+Qed.
+          
+Theorem type_of_correct : forall t : term, forall e : env,
+                            match type_of e t with
+                              | Some ty => typing e t ty
+                              | None => forall ty : typ, typing e t ty -> False
+                            end.
+  intro.
+  induction t.
+  + (* var *) {
+      intro. simpl.
+      case (get_typ e n).
+      - {
+          intro. unfold wf_env. case (bwf_env e).
+          auto.
+          intros. destruct H. discriminate H.
+        }
+      - case (bwf_env e). auto. auto.
+    }
+  + (* abs *) {
+      intro.
+      simpl.
+      specialize (IHt (evar t e)).
+      remember (type_of (evar t e) t0) as ty in IHt |- *.
+      destruct ty.
+      - split. auto. apply IHt.
+      - {
+          intro.
+          destruct ty.
+          * auto.
+          * {
+              intro.
+              destruct H.
+              apply IHt with (ty := ty2).
+              rewrite <- H.
+              apply H0.
+            }
+          * auto.
+        }
+    }
+  + (* app *) {
+      intro.
+      specialize (IHt1 e).
+      specialize (IHt2 e).
+      simpl.
+      remember (type_of e t1) as ty1 in IHt1 |- *.
+      remember (type_of e t2) as ty2 in IHt2 |- *.
+      destruct ty1.
+      destruct ty2.
+      - {
+          destruct t.
+          * {
+              intros.
+              destruct H. destruct H.
+              Check typing_uniq.
+              apply (typing_uniq t1 e (tvar n) (tarr x ty)) in IHt1.
+              discriminate IHt1.
+              apply H.
+            }
+          * {
+              remember (beq_typ t3 t0) as beqt in *.
+              destruct beqt.
+              - {
+                  exists t3.
+                  split.
+                  apply IHt1.
+                  apply eq_sym in Heqbeqt. apply beq_typ_correct in Heqbeqt.
+                  rewrite -> Heqbeqt. apply IHt2.
+                }
+              - {
+                  intros.
+                  destruct H.
+                  destruct H.
+                  Check typing_uniq.
+                  apply (typing_uniq t2 e t0 x) in IHt2.
+                  apply (typing_uniq t1 e (tarr t3 t4) (tarr x ty)) in IHt1.
+                  inversion IHt1.
+                  apply eq_sym in IHt2. apply (eq_trans H2) in IHt2.
+                  rewrite <- IHt2 in Heqbeqt. 
+                  pose proof beq_typ_refl as EqRefl.
+                  specialize (EqRefl t3).
+                  apply (eq_trans Heqbeqt) in EqRefl. inversion EqRefl.
+                  apply H.
+                  apply H0.
+                }
+            }
+          * {
+              intros.
+              destruct H. destruct H.
+              apply (typing_uniq t1 e (tall k t) (tarr x ty)) in IHt1.
+              inversion IHt1.
+              apply H.
+            }
+        }
+      - {
+          destruct t.
+          * intros. destruct H. apply (IHt2 x). apply H.
+          * intros. destruct H. apply (IHt2 x). apply H.
+          * intros. destruct H. apply (IHt2 x). apply H.
+        }
+      - {
+          intros.
+          destruct H.
+          apply (IHt1 (tarr x ty)).
+          apply H.
+        }
+    }
+  + (* abs_t *) {
+      intros.
+      simpl.
+      remember (type_of (etvar k e) t) as ty1.
+      specialize (IHt (etvar k e)).
+      destruct ty1.
+      - {
+          split. auto.
+          rewrite <- Heqty1 in IHt.
+          apply IHt.
+        }
+      - {
+          rewrite <- Heqty1 in IHt.
+          intro. destruct ty.
+          auto.
+          auto.
+          intro.
+          apply (IHt ty).
+          apply H.
+        }
+    }
+  + (* app_t *) {
+      intros.
+      simpl.   
+      specialize (IHt e).
+      remember (type_of e t) as ty in IHt |- *.
+      destruct ty.
+      destruct t1.
+      - {
+          intros.
+          destruct H. destruct H. destruct H.
+          apply (typing_uniq t e (tvar n) (tall x x0)) in IHt. inversion IHt. apply H.
+        }
+      - {
+          intros. destruct H. destruct H. destruct H.
+          apply (typing_uniq t e (tarr t1_1 t1_2) (tall x x0)) in IHt. inversion IHt. apply H.
+        }
+      - {
+          remember (kind_of e t0) as k0 in *.
+          destruct k0.
+          remember (leq k0 k) as lk0.
+          destruct lk0.
+          * {
+              exists k. exists t1. split. apply IHt. split.
+              pose proof (kind_of_correct t0 e). rewrite <- Heqk0 in H.
+              apply (kinding_sub t0 e k0 k).
+              apply leq_prop. apply Heqlk0.
+              apply H.
+              reflexivity.
+            }
+          * {
+              intros.
+              destruct H. destruct H. destruct H. destruct H0.
+              pose proof kind_of_minimal.
+              specialize (H2 t0 e x).
+              rewrite <- Heqk0 in H2.
+              apply H2 in H0.
+              pose proof (typing_uniq t e (tall k t1) (tall x x0) IHt H).
+              inversion H3.
+              pose proof (leq_prop k0 k).
+              destruct H4.
+              rewrite <- H5 in H0. apply H7 in H0. apply eq_sym in H0. apply (eq_trans Heqlk0) in H0.
+              discriminate H0.
+            }
+          * {
+              intros.
+              destruct H. destruct H. destruct H. destruct H0.
+              Check kind_of_correct.
+              pose proof (kind_of_correct t0 e).
+              rewrite <- Heqk0 in H2. apply H2 in H0. apply H0.
+            }
+        }
+      - intros. destruct H. destruct H. destruct H. apply (IHt (tall x x0)). apply H.
+    }
+Qed.
+
+          
